CollapsingTowers/TwoLevel/LR.lean
@@ -7,13 +7,16 @@ import CollapsingTowers.TwoLevel.Env
 import CollapsingTowers.TwoLevel.Typing
 
 @[simp]
+def wf (e : Expr) : Prop := closedb_at e 0 ∧ closed_at e 0
+
+@[simp]
 def valType : Expr → Ty → Prop
   | .lam₁ t2, .arrow τ1 τ2 =>
     ∀ v1, valType v1 τ1 ∧ lc v1 →
-    ∃ v2, stepn (open_subst v1 t2) v2 ∧ valType v2 τ2
+    ∃ v2, stepn (open_subst v1 t2) v2 ∧ closedb_at v2 0 ∧ valType v2 τ2
   | .lit₁ _, .nat => true
   | .code e, .rep τ =>
-    ∃ v, stepn e v ∧ valType v τ
+    ∃ v, stepn e v ∧ wf e ∧ valType v τ
   | _, _ => false
 
 @[simp]
@@ -33,7 +36,8 @@ theorem envType.extend : ∀ Δ Γ v τ,
   . apply henv.1
   . intros τ1 x bd; rcases henv with ⟨hlen, h⟩
     by_cases hx : (x = Γ.length)
-    . rw [hx] at bd; simp at bd; rw [hlen]; simp [hx]; rw [<- bd]; apply And.intro; assumption; assumption
+    . rw [hx] at bd; simp at bd; rw [hlen]; simp [hx]; rw [<- bd];
+      apply And.intro; assumption; assumption
     . rw [if_neg hx] at bd; rw [hlen]; rw [if_neg hx]
       apply h; assumption
 
@@ -43,7 +47,7 @@ theorem envType.closed : ∀ Δ Γ,
   have hx : (x < Δ.length) := by apply indexrSome'; exists t1
   rw [hlen] at hx; have hidx' := indexrSome Γ x hx
   rcases hidx' with ⟨τ, hidx'⟩
-  have ⟨t2, hidx'', hval⟩  := h τ x hidx'
+  have ⟨t2, hidx'', hval⟩ := h τ x hidx'
   rcases hval with ⟨hcl, _⟩; rw [hidx] at hidx''; cases hidx''; assumption
 
 @[simp]
@@ -73,7 +77,7 @@ def semType (Γ : TEnv) (t : Expr) (τ : Ty) : Prop :=
   ∀ Δ, lc t → envType Δ Γ → expType (substF Δ t) τ
 
 lemma substF.closedb_at: ∀ t Δ n,
-  (forall x t1, indexr x Δ = some t1 -> closedb_at t1 0) ->
+  (∀ x t1, indexr x Δ = some t1 -> closedb_at t1 0) ->
   (closedb_at t n) -> (closedb_at (substF Δ t) n) := by
   intros t; induction t <;> intros E n hidx hcl <;> simp
   case bvar x => simp at hcl; assumption
@@ -98,6 +102,37 @@ lemma substF.closedb_at: ∀ t Δ n,
     . apply ih1; assumption; assumption
     . apply ih2; assumption; assumption
 
+lemma substF_opening_comm: ∀ t t1 Δ n, closed_at t Δ.length →
+  (∀ x t1, indexr x Δ = some t1 → closedb_at t1 0) →
+  substF (t1::Δ) (opening n (.fvar Δ.length) t) =
+  opening n t1 (substF Δ t) := by
+  intros t t1 Δ n h; revert n; induction t <;> intros n hc <;> simp
+  case bvar x =>
+    by_cases hx: (x = n)
+    simp [hx]; rw [if_neg hx]; rw [if_neg hx]; simp
+  case fvar x =>
+    have h' := indexrSome Δ x h
+    rcases h' with ⟨v, hidx⟩; rw [hidx]; simp;
+    have hx : ¬(x = Δ.length) := by simp at h; omega
+    rw [if_neg hx]; simp;
+    rw [closedb_opening_id]; apply closedb_inc; apply hc; apply hidx; omega
+  case lam₁ t ih
+     | lam₂ t ih =>
+    apply ih; simp at h; assumption; assumption
+  case code _ ih
+     | reflect _ ih
+     | lam𝕔 _ ih =>
+    apply ih; assumption; assumption
+  case app₁ t1 t2 ih1 ih2
+     | app₂ t1 t2 ih1 ih2
+     | plus₁ _ _ ih1 ih2
+     | plus₂ _ _ ih1 ih2
+     | lets _ _ ih1 ih2
+     | let𝕔 _ _ ih1 ih2 =>
+    simp at h; apply And.intro
+    . apply ih1; apply h.1; assumption
+    . apply ih2; apply h.2; assumption
+
 -- compatibility lemmas
 
 lemma semType.fvar: ∀ Γ x τ, binds x τ Γ → semType Γ (.fvar x) τ := by
@@ -108,16 +143,31 @@ lemma semType.fvar: ∀ Γ x τ, binds x τ Γ → semType Γ (.fvar x) τ := by
 
 lemma semType.lam₁: ∀ Γ e τ1 τ2,
   semType (τ1 :: Γ) (open₀ Γ.length e) τ2 →
-  Γ.length ∉ fv e ->
+  closed_at e Γ.length →
   semType Γ (.lam₁ e) (.arrow τ1 τ2) := by
   intros Γ e τ1 τ2 hsem hfr Δ hcl henv
   exists (substF Δ (.lam₁ e));
   constructor; apply stepn.refl
-  constructor; sorry
-  sorry
+  have hcl' := open_closed' e (Γ.length) 0 hcl
+  constructor; apply substF.closedb_at; apply envType.closed; assumption; assumption
+  simp; intros v1 hv1 hclv1;
+  have henv' := envType.extend Δ Γ v1 τ1 henv hclv1 hv1
+  have hsem' := hsem (v1::Δ) hcl' henv'
+  rcases hsem' with ⟨vy, hyst, semvy⟩
+  exists vy; apply And.intro
+  . rw [<-henv.1] at hyst
+    rw [open₀, substF_opening_comm] at hyst; assumption
+    rw [henv.1]; assumption; apply envType.closed Δ Γ henv
+  . assumption
 
 lemma semType.lam₂: ∀ Γ e τ1 τ2,
   semType (.rep τ1 :: Γ) (open₀ Γ.length e) τ2 →
-  Γ.length ∉ fv e ->
+  closed_at e Γ.length →
   semType Γ (.lam₂ e) (.rep (.arrow τ1 τ2)) := by
+  intros Γ e τ1 τ2 hsem hfr Δ hcl henv
+  unfold semType at hsem
+  unfold expType at *
+  have var : Expr := .fvar (Γ.length)
+  have Δ' := var::Δ
+  have Γ' := τ1.rep :: Γ
   sorry
